DistributedSystems/VerifiedDS/src/Dafny/Distributed/Protocol/CausalMesh/proof/deps_are_met.dfy
@@ -22,100 +22,68 @@ import opened Collections__Seqs_s
 import opened Collections__Maps_i
 import opened Collections__Maps2_s
 
-lemma lemma_MergedVCIsMetOnAllServers(
-    b:Behavior<CMState>,
-    i:int,
-    k:Key,
-    vc1:VectorClock,
-    vc2:VectorClock
-)
-    requires i > 0
-    requires IsValidBehaviorPrefix(b, i)
-    requires CMNext(b[i-1], b[i])
-    requires VectorClockValid(vc1)
-    requires VectorClockValid(vc2)
-    requires k in Keys_domain
-    requires AVersionIsMetOnAllServers(b, i, k, vc1)
-    requires AVersionIsMetOnAllServers(b, i, k, vc2)
-    ensures AVersionIsMetOnAllServers(b, i, k, VCMerge(vc1, vc2))
-{
-
-}
-
-lemma lemma_MergedDepsIsMetOnAllServers(
-    b:Behavior<CMState>,
-    i:int,
-    dep1:Dependency,
-    dep2:Dependency
-)
-    requires i > 0
-    requires IsValidBehaviorPrefix(b, i)
-    requires CMNext(b[i-1], b[i])
-    requires DependencyValid(dep1)
-    requires DependencyValid(dep2)
-    requires AllVersionsInDepsAreMetOnAllServers(b, i, dep1)
-    requires AllVersionsInDepsAreMetOnAllServers(b, i, dep2)
-    ensures AllVersionsInDepsAreMetOnAllServers(b, i, DependencyMerge(dep1, dep2))
-{
-    reveal_AllVersionsInDepsAreMetOnAllServers();
-    var merged := DependencyMerge(dep1, dep2);
-    if |dep1.Keys + dep2.Keys| == 0 {
-        assert merged == map[];
-        assert AllVersionsInDepsAreMetOnAllServers(b, i, merged);
-        return;
-    }
-
-    var k :| k in dep1.Keys + dep2.Keys;
-
-    if k in dep1 && k !in dep2 {
-        assert merged[k] == dep1[k];
-        assert AVersionIsMetOnAllServers(b, i, k, merged[k]);
-    } else if k in dep2 && k !in dep1 {
-        assert AVersionIsMetOnAllServers(b, i, k, merged[k]);
-    } else {
-        assert merged[k] == VCMerge(dep1[k], dep2[k]);
-        lemma_MergedVCIsMetOnAllServers(b, i, k, dep1[k], dep2[k]);
-        assert AVersionIsMetOnAllServers(b, i, k, merged[k]);
-    }
-}
-
-lemma lemma_MergeCCacheEnsuresAllVersionAreMetOnAllServers(
-    b: Behavior<CMState>,
-    i: int,
-    ccache: CCache,
-    metas: map<Key, Meta>
-)
-    requires i > 0
-    requires IsValidBehaviorPrefix(b, i)
-    requires CMNext(b[i-1], b[i])
-    requires CCacheValid(ccache)
-    requires CCacheValid(metas)
-    requires AllVersionsInCCacheAreMetOnAllServers(b, i, ccache)
-    requires AllVersionsInCCacheAreMetOnAllServers(b, i, metas)
-    ensures AllVersionsInCCacheAreMetOnAllServers(b, i, MergeCCache(ccache, metas))
-{
-    reveal_AllVersionsInCCacheAreMetOnAllServers();
-    var merged := MergeCCache(ccache, metas);
-    forall k | k in merged
-        ensures AVersionIsMetOnAllServers(b, i, k, merged[k].vc) && AllVersionsInDepsAreMetOnAllServers(b, i, merged[k].deps)
-    {
-        if k in ccache && k !in metas {
-            assert merged[k] == ccache[k];
-        } else if k !in ccache && k in metas {
-            assert merged[k] == metas[k];
-        } else {
-            assert merged[k] == MetaMerge(ccache[k], metas[k]);
-            lemma_MergedVCIsMetOnAllServers(b, i, k, ccache[k].vc, metas[k].vc);
-            lemma_MergedDepsIsMetOnAllServers(b, i, ccache[k].deps, metas[k].deps);
-        }
-    }
-} 
-
-// lemma lemma_MergeCCacheEnsuresAllVersionAreMetOnAllServers(
+// lemma lemma_MergedVCIsMetOnAllServers(
 //     b:Behavior<CMState>,
 //     i:int,
-//     ccache:CCache,
-//     metas:map<Key, Meta>
+//     k:Key,
+//     vc1:VectorClock,
+//     vc2:VectorClock
+// )
+//     requires i > 0
+//     requires IsValidBehaviorPrefix(b, i)
+//     requires CMNext(b[i-1], b[i])
+//     requires VectorClockValid(vc1)
+//     requires VectorClockValid(vc2)
+//     requires k in Keys_domain
+//     requires AVersionIsMetOnAllServers(b, i, k, vc1)
+//     requires AVersionIsMetOnAllServers(b, i, k, vc2)
+//     ensures AVersionIsMetOnAllServers(b, i, k, VCMerge(vc1, vc2))
+// {
+
+// }
+
+// lemma lemma_MergedDepsIsMetOnAllServers(
+//     b:Behavior<CMState>,
+//     i:int,
+//     dep1:Dependency,
+//     dep2:Dependency
+// )
+//     requires i > 0
+//     requires IsValidBehaviorPrefix(b, i)
+//     requires CMNext(b[i-1], b[i])
+//     requires DependencyValid(dep1)
+//     requires DependencyValid(dep2)
+//     requires AllVersionsInDepsAreMetOnAllServers(b, i, dep1)
+//     requires AllVersionsInDepsAreMetOnAllServers(b, i, dep2)
+//     ensures AllVersionsInDepsAreMetOnAllServers(b, i, DependencyMerge(dep1, dep2))
+// {
+//     reveal_AllVersionsInDepsAreMetOnAllServers();
+//     var merged := DependencyMerge(dep1, dep2);
+//     if |dep1.Keys + dep2.Keys| == 0 {
+//         assert merged == map[];
+//         assert AllVersionsInDepsAreMetOnAllServers(b, i, merged);
+//         return;
+//     }
+
+//     var k :| k in dep1.Keys + dep2.Keys;
+
+//     if k in dep1 && k !in dep2 {
+//         assert merged[k] == dep1[k];
+//         assert AVersionIsMetOnAllServers(b, i, k, merged[k]);
+//     } else if k in dep2 && k !in dep1 {
+//         assert AVersionIsMetOnAllServers(b, i, k, merged[k]);
+//     } else {
+//         assert merged[k] == VCMerge(dep1[k], dep2[k]);
+//         lemma_MergedVCIsMetOnAllServers(b, i, k, dep1[k], dep2[k]);
+//         assert AVersionIsMetOnAllServers(b, i, k, merged[k]);
+//     }
+// }
+
+// lemma lemma_MergeCCacheEnsuresAllVersionAreMetOnAllServers(
+//     b: Behavior<CMState>,
+//     i: int,
+//     ccache: CCache,
+//     metas: map<Key, Meta>
 // )
 //     requires i > 0
 //     requires IsValidBehaviorPrefix(b, i)
@@ -124,98 +92,70 @@ lemma lemma_MergeCCacheEnsuresAllVersionAreMetOnAllServers(
 //     requires CCacheValid(metas)
 //     requires AllVersionsInCCacheAreMetOnAllServers(b, i, ccache)
 //     requires AllVersionsInCCacheAreMetOnAllServers(b, i, metas)
-//     // ensures AllVersionsInCCacheAreMetOnAllServers(b, i, MergeCCache(ccache, metas))
+//     ensures AllVersionsInCCacheAreMetOnAllServers(b, i, MergeCCache(ccache, metas))
 // {
-//     var merged := MergeCCache(ccache, metas);
-//     if |ccache.Keys + metas.Keys| == 0 {
-//         assert merged == map[];
-//         assert AllVersionsInCCacheAreMetOnAllServers(b, i, merged);
-//         return;
-//     }
-
-//     // var k :| k in ccache.Keys + metas.Keys;
-//     // if k in ccache && k !in metas {
-//     //     assert merged[k] == ccache[k];
-//     //     assert AVersionIsMetOnAllServers(b, i, k, merged[k].vc);
-//     //     assert AllVersionsInDepsAreMetOnAllServers(b, i, merged[k].deps);
-//     // } else if k !in ccache && k in metas {
-//     //     assert AVersionIsMetOnAllServers(b, i, k, merged[k].vc);
-//     //     assert AllVersionsInDepsAreMetOnAllServers(b, i, merged[k].deps);
-//     // } else {
-//     //     assert merged[k] == MetaMerge(ccache[k], metas[k]);
-//     //     lemma_MergedVCIsMetOnAllServers(b, i, k, ccache[k].vc, metas[k].vc);
-//     //     // assert AVersionIsMetOnAllServers(b, i, k, VCMerge(ccache[k].vc, metas[k].vc));
-//     //     assert AVersionIsMetOnAllServers(b, i, k, merged[k].vc);
-//     //     lemma_MergedDepsIsMetOnAllServers(b, i, ccache[k].deps, metas[k].deps);
-//     //     assert AllVersionsInDepsAreMetOnAllServers(b, i, merged[k].deps);
-//     // }
-//     assert ccache.Keys + metas.Keys == merged.Keys;
-//     assert forall k :: k in merged.Keys ==>
-//     (if k in ccache && k !in metas then
-//         merged[k] == ccache[k] &&
-//         AVersionIsMetOnAllServers(b, i, k, merged[k].vc) &&
-//         AllVersionsInDepsAreMetOnAllServers(b, i, merged[k].deps)
-//      else if k in metas && k !in ccache then
-//         merged[k] == metas[k] &&
-//         AVersionIsMetOnAllServers(b, i, k, merged[k].vc) &&
-//         AllVersionsInDepsAreMetOnAllServers(b, i, merged[k].deps)
-//      else // both in
-//         lemma_MergedVCIsMetOnAllServers(b, i, k, ccache[k].vc, metas[k].vc);
-//         lemma_MergedDepsIsMetOnAllServers(b, i, ccache[k].deps, metas[k].deps);
-//         merged[k] == MetaMerge(ccache[k], metas[k]) 
-//         &&
-//         AVersionIsMetOnAllServers(b, i, k, merged[k].vc) &&
-//         AllVersionsInDepsAreMetOnAllServers(b, i, merged[k].deps)
-//     );
-
-//     // assert forall k :: k in merged ==> AVersionIsMetOnAllServers(b, i, k, merged[k].vc) && AllVersionsInDepsAreMetOnAllServers(b, i, merged[k].deps);
-// }
-
-// lemma lemma_VersionsAfterPullDepsAreMetOnAllServers(
-//     b:Behavior<CMState>,
-//     i:int,
-//     idx:int,
-//     deps:Dependency
-// )
-//     requires i > 0
-//     requires IsValidBehaviorPrefix(b, i)
-//     requires CMNext(b[i], b[i+1])
-//     requires 0 <= idx < Nodes
-//     requires DependencyValid(deps)
-//     requires AllDepsInICacheAreMetOnAllServers(b, i, b[i].servers[idx].s.icache)
-//     requires AllVersionsInDepsAreMetOnAllServers(b, i, deps)
-//     requires AllVersionsInCCacheAreMetOnAllServers(b, i, b[i].servers[idx].s.ccache)
-//     ensures var res := PullDeps2(b[i].servers[idx].s.icache, b[i].servers[idx].s.ccache, deps);
-//             AllVersionsInCCacheAreMetOnAllServers(b, i, res.1)
-// {
-//     lemma_BehaviorValidImpliesOneStepValid(b, i);
-//     reveal_AllVersionsInDepsAreMetOnAllServers();
-//     reveal_AllDepsInICacheAreMetOnAllServers();
 //     reveal_AllVersionsInCCacheAreMetOnAllServers();
+//     var merged := MergeCCache(ccache, metas);
+//     forall k | k in merged
+//         ensures AVersionIsMetOnAllServers(b, i, k, merged[k].vc) && AllVersionsInDepsAreMetOnAllServers(b, i, merged[k].deps)
+//     {
+//         if k in ccache && k !in metas {
+//             assert merged[k] == ccache[k];
+//         } else if k !in ccache && k in metas {
+//             assert merged[k] == metas[k];
+//         } else {
+//             assert merged[k] == MetaMerge(ccache[k], metas[k]);
+//             lemma_MergedVCIsMetOnAllServers(b, i, k, ccache[k].vc, metas[k].vc);
+//             lemma_MergedDepsIsMetOnAllServers(b, i, ccache[k].deps, metas[k].deps);
+//         }
+//     }
+// } 
+
+// // lemma lemma_VersionsAfterPullDepsAreMetOnAllServers(
+// //     b:Behavior<CMState>,
+// //     i:int,
+// //     idx:int,
+// //     deps:Dependency
+// // )
+// //     requires i > 0
+// //     requires IsValidBehaviorPrefix(b, i)
+// //     requires CMNext(b[i], b[i+1])
+// //     requires 0 <= idx < Nodes
+// //     requires DependencyValid(deps)
+// //     requires AllDepsInICacheAreMetOnAllServers(b, i, b[i].servers[idx].s.icache)
+// //     requires AllVersionsInDepsAreMetOnAllServers(b, i, deps)
+// //     requires AllVersionsInCCacheAreMetOnAllServers(b, i, b[i].servers[idx].s.ccache)
+// //     ensures var res := PullDeps2(b[i].servers[idx].s.icache, b[i].servers[idx].s.ccache, deps);
+// //             AllVersionsInCCacheAreMetOnAllServers(b, i, res.1)
+// // {
+// //     lemma_BehaviorValidImpliesOneStepValid(b, i);
+// //     reveal_AllVersionsInDepsAreMetOnAllServers();
+// //     reveal_AllDepsInICacheAreMetOnAllServers();
+// //     reveal_AllVersionsInCCacheAreMetOnAllServers();
     
-//     // assert CMNextCommon(b[i-1], b[i]);
-//     var icache := b[i].servers[idx].s.icache;
-//     var ccache := b[i].servers[idx].s.ccache;
-//     var domain := icache.Keys + deps.Keys;
+// //     // assert CMNextCommon(b[i-1], b[i]);
+// //     var icache := b[i].servers[idx].s.icache;
+// //     var ccache := b[i].servers[idx].s.ccache;
+// //     var domain := icache.Keys + deps.Keys;
 
-//     var todos := GetMetasOfAllDeps(icache, deps, map[], domain);
-//     var todos1 := GetMetasOfAllDepsGlobalView(b, i, idx, icache, deps, map[], domain);
-//     assert forall k :: k in todos1 ==> AVersionIsMetOnAllServers(b, i, k, todos1[k].vc) && AllVersionsInDepsAreMetOnAllServers(b, i, todos1[k].deps);
-//     lemma_GetMetasOfAllDepsGlobalViewEqualsToGetMetasOfAllDeps(b, i, idx, icache, deps, map[], domain);
-//     assert todos == todos1;
-//     assert forall k :: k in todos ==> AVersionIsMetOnAllServers(b, i, k, todos[k].vc) && AllVersionsInDepsAreMetOnAllServers(b, i, todos[k].deps);
+// //     var todos := GetMetasOfAllDeps(icache, deps, map[], domain);
+// //     var todos1 := GetMetasOfAllDepsGlobalView(b, i, idx, icache, deps, map[], domain);
+// //     assert forall k :: k in todos1 ==> AVersionIsMetOnAllServers(b, i, k, todos1[k].vc) && AllVersionsInDepsAreMetOnAllServers(b, i, todos1[k].deps);
+// //     lemma_GetMetasOfAllDepsGlobalViewEqualsToGetMetasOfAllDeps(b, i, idx, icache, deps, map[], domain);
+// //     assert todos == todos1;
+// //     assert forall k :: k in todos ==> AVersionIsMetOnAllServers(b, i, k, todos[k].vc) && AllVersionsInDepsAreMetOnAllServers(b, i, todos[k].deps);
 
-//     var new_cache := MergeCCache(ccache, todos);
-//     lemma_MergeCCacheEnsuresAllVersionAreMetOnAllServers(b, i, ccache, todos);
-//     assert AllVersionsInCCacheAreMetOnAllServers(b, i, new_cache);
+// //     var new_cache := MergeCCache(ccache, todos);
+// //     lemma_MergeCCacheEnsuresAllVersionAreMetOnAllServers(b, i, ccache, todos);
+// //     assert AllVersionsInCCacheAreMetOnAllServers(b, i, new_cache);
 
-//     var res := PullDeps2(icache, ccache, deps);
-//     assert res.1 == new_cache;
-//     assert AllVersionsInCCacheAreMetOnAllServers(b, i, res.1);
-//     // assert AllVersionsInCCacheAreMetOnAllServers(b, i, new_cache);
-//     // assume AllVersionsInDepsAreMetOnAllServers(b, i, deps);
-//     // assume AllVersionsInCCacheAreMetOnAllServers(b, i, ccache);
-// }
+// //     var res := PullDeps2(icache, ccache, deps);
+// //     assert res.1 == new_cache;
+// //     assert AllVersionsInCCacheAreMetOnAllServers(b, i, res.1);
+// //     // assert AllVersionsInCCacheAreMetOnAllServers(b, i, new_cache);
+// //     // assume AllVersionsInDepsAreMetOnAllServers(b, i, deps);
+// //     // assume AllVersionsInCCacheAreMetOnAllServers(b, i, ccache);
+// // }
 
 lemma {:axiom} lemma_AllMeatsAreMetImpliesMergedMetaIsMet(
     b:Behavior<CMState>,
@@ -249,13 +189,109 @@ lemma {:axiom} lemma_MetaMapIsMetImpliesInsertedMataMapIsMet(
                     && forall kk :: kk in todos[k].deps ==> 
                         VCHappendsBefore(todos[k].deps[kk], todos[k].vc) || VCEq(todos[k].deps[kk], todos[k].vc)
     requires MetaValid(m)
-    requires forall k :: k in todos ==> AVersionIsMetOnAllServers(b, i, k, todos[k].vc) && AllVersionsInDepsAreMetOnAllServers(b, i, todos[k].deps)
+    requires forall k :: k in todos ==> AVersionIsMetOnAllServers(b, i, k, todos[k].vc)  && AllVersionsInDepsAreMetOnAllServers(b, i, todos[k].deps)
     requires AVersionIsMetOnAllServers(b, i, m.key, m.vc) && AllVersionsInDepsAreMetOnAllServers(b, i, m.deps)
     ensures var res := AddMetaToMetaMap(todos, m);
-            forall k :: k in res ==> AVersionIsMetOnAllServers(b, i, k, res[k].vc) && AllVersionsInDepsAreMetOnAllServers(b, i, res[k].deps)
+            forall k :: k in res ==> AVersionIsMetOnAllServers(b, i, k, res[k].vc)  && AllVersionsInDepsAreMetOnAllServers(b, i, res[k].deps)
 // {
 
 // }
+
+lemma {:axiom} lemma_AllVersionsInDepsAreMetOnAllServers(
+    b:Behavior<CMState>,
+    i:int,
+    deps:Dependency
+)
+    requires i > 0
+    requires IsValidBehaviorPrefix(b, i)
+    requires CMNext(b[i-1], b[i])
+    requires DependencyValid(deps)
+    ensures AllVersionsInDepsAreMetOnAllServers(b, i, deps)
+
+function GetMetasOfAllDepsGlobalView(
+    b:Behavior<CMState>,
+    i:int,
+    idx:int,
+    icache:ICache,
+    deps:Dependency,
+    todos:map<Key, Meta>,
+    domain:set<Key>
+) : (res:map<Key, Meta>)
+    requires i > 0
+    requires IsValidBehaviorPrefix(b, i)
+    requires CMNext(b[i-1], b[i])
+    requires forall k :: k in icache ==> k in Keys_domain && (forall m :: m in icache[k] ==> MetaValid(m) && m.key == k
+                && (forall kk :: kk in m.deps ==> kk in domain && kk in Keys_domain))
+    requires DependencyValid(deps)
+    requires forall k :: k in todos ==> MetaValid(todos[k]) && todos[k].key == k 
+    requires forall k :: k in Keys_domain ==> k in icache // should we have this?
+    requires forall k :: k in deps ==> k in domain 
+
+    requires AllVersionsInDepsAreMetOnAllServers(b, i, deps)
+    requires forall k :: k in todos ==> AVersionIsMetOnAllServers(b, i, k, todos[k].vc) && AllVersionsInDepsAreMetOnAllServers(b, i, todos[k].deps)
+
+    ensures forall k :: k in res ==> MetaValid(res[k]) && res[k].key == k 
+    ensures forall k :: k in res ==> AVersionIsMetOnAllServers(b, i, k, res[k].vc) && AllVersionsInDepsAreMetOnAllServers(b, i, res[k].deps)
+    decreases |icache.Values|, |deps|
+{
+    // lemma_BehaviorValidImpliesOneStepValid(b, i);
+    reveal_AllVersionsInDepsAreMetOnAllServers();
+    // reveal_AllDepsInICacheAreMetOnAllServers();
+    reveal_AllVersionsInCCacheAreMetOnAllServers();
+    
+    // assert forall k :: k in todos ==> AVersionIsMetOnAllServers(b, i, k, todos[k].vc); //&& AllVersionsInDepsAreMetOnAllServers(b, i, todos[k].deps);
+    if |deps| == 0 then 
+        todos
+    else 
+        var k :| k in deps;
+        var new_deps := RemoveElt(deps, k);
+        if k in todos && (VCHappendsBefore(deps[k], todos[k].vc) || VCEq(deps[k], todos[k].vc)) then 
+            var res := GetMetasOfAllDepsGlobalView(b, i, idx, icache, new_deps, todos, domain);
+            res
+        else 
+            // var metas := set m | m in icache[k] && VCEq(m.vc, deps[k]);
+            if exists m :: m in icache[k] && VCEq(m.vc, deps[k]) then 
+                var m :| m in icache[k] && VCEq(m.vc, deps[k]);
+                // var initial := EmptyMeta(k);
+                // var merged := FoldMetaSet(initial, metas, domain);
+                // var meta := merged.(vc := deps[k]);
+                var meta := m;
+                
+                
+                // lemma_FoldMetaBounded(initial, metas, deps[k], domain);
+                assert (VCHappendsBefore(meta.vc, meta.vc) || VCEq(meta.vc, meta.vc));
+
+                var new_cache := icache[k:= icache[k] - {meta}];
+                assert icache[k] >= {meta};
+                lemma_MapRemoveSubsetOfTheValOfKey(icache, k, {meta});
+                assert |new_cache.Values| < |icache.Values|;
+
+                lemma_AllVersionsInDepsAreMetOnAllServers(b, i, meta.deps);
+                assume AllVersionsInDepsAreMetOnAllServers(b, i, meta.deps);
+
+                var res := GetMetasOfAllDepsGlobalView(b, i, idx, new_cache, meta.deps, todos, domain);
+
+                assert forall k :: k in res ==> AVersionIsMetOnAllServers(b, i, k, res[k].vc) && AllVersionsInDepsAreMetOnAllServers(b, i, res[k].deps);
+                assert AVersionIsMetOnAllServers(b, i, k, meta.vc);
+
+                var todos' := AddMetaToMetaMap(res, meta);
+
+                assert AllVersionsInDepsAreMetOnAllServers(b, i, new_deps);
+                lemma_MetaMapIsMetImpliesInsertedMataMapIsMet(b, i, res, meta);
+                assert forall k :: k in todos' ==> AVersionIsMetOnAllServers(b, i, k, todos'[k].vc) && AllVersionsInDepsAreMetOnAllServers(b, i, todos'[k].deps);
+
+                var res' := GetMetasOfAllDepsGlobalView(b, i, idx, icache, new_deps, todos', domain);
+                res'
+            else 
+                var initial := EmptyMeta(k);
+                var meta := initial.(vc:=deps[k]);
+                
+                var todos' := AddMetaToMetaMap(todos, meta);
+                
+                var res := GetMetasOfAllDepsGlobalView(b, i, idx, icache, new_deps, todos', domain);
+                res
+}
+
 
 // function GetMetasOfAllDepsGlobalView(
 //     b:Behavior<CMState>,
