DistributedSystems/VerifiedDS/src/Dafny/Distributed/Protocol/CausalMesh/proof/packet_sending.dfy
@@ -33,6 +33,7 @@ lemma lemma_ActionThatSendsReadReplyIsServerReceiveRead(
     ensures ios[0].LIoOpReceive?
     ensures ios[0].r.msg.Message_Read?
     ensures LIoOpSend(p) in ios
+    // ensures ios[0].r.dst == idx
     ensures ReceiveRead(ps.servers[idx].s, ps'.servers[idx].s, ios[0].r, [p])
 {
     assert ps.environment.nextStep.LEnvStepHostIos?;
@@ -79,6 +80,7 @@ lemma lemma_ActionThatSendsWriteReplyIsServerReceiveWrite(
     ensures ios[0].LIoOpReceive?
     ensures ios[0].r.msg.Message_Write?
     ensures LIoOpSend(p) in ios
+    // ensures ios[0].r.dst == idx
     ensures ReceiveWrite(ps.servers[idx].s, ps'.servers[idx].s, ios[0].r, ExtractSentPacketsFromIos(ios))
 {
     assert ps.environment.nextStep.LEnvStepHostIos?;
@@ -155,6 +157,7 @@ lemma lemma_ActionThatSendsPropagationIsReceivePropogateOrReceiveWrite(
     ensures ios[0].LIoOpReceive?
     ensures ios[0].r.msg.Message_Write? || ios[0].r.msg.Message_Propagation?
     ensures LIoOpSend(p) in ios
+    // ensures ios[0].r.dst == idx
     ensures ios[0].r.msg.Message_Propagation? ==> ReceivePropagate(ps.servers[idx].s, ps'.servers[idx].s, ios[0].r, ExtractSentPacketsFromIos(ios))
     ensures ios[0].r.msg.Message_Write? ==> ReceiveWrite(ps.servers[idx].s, ps'.servers[idx].s, ios[0].r, ExtractSentPacketsFromIos(ios))
 {
