DistributedSystems/VerifiedDS/src/Dafny/Distributed/Protocol/CausalMesh/proof/propagation.dfy
@@ -25,90 +25,202 @@ import opened Collections__Maps_i
 import opened Collections__Maps2_s
 
 
-// lemma lemma_PropagationAtTail(
-//     b:Behavior<CMState>,
-//     i:int,
-//     idx:int,
-//     p:Packet,
-//     ios:seq<CMIo>
-// )
-//     requires 0 < i 
-//     requires IsValidBehaviorPrefix(b, i)
-//     requires forall j :: 0 <= j < i ==> CMNext(b[j], b[j+1])
-//     requires CMNext(b[i-1], b[i])
-//     requires 0 <= idx < Nodes
-//     requires |ios| > 1
-//     requires ios[0].LIoOpReceive?
-//     requires p.msg.Message_Propagation?
-//     requires p in b[i-1].environment.sentPackets
-//     requires p.dst == idx
-//     requires idx == b[i-1].servers[idx].s.id
-//     requires ios[0].r == p
-//     requires PacketValid(p)
-//     requires p.msg.start == b[i-1].servers[idx].s.next
-//     requires ReceivePropagate(b[i-1].servers[idx].s, b[i].servers[idx].s, p, ExtractSentPacketsFromIos(ios))
-//     ensures AVersionIsMetOnAllServers(b, i, ios[0].r.msg.key, ios[0].r.msg.meta.vc)
-// {
-//     var p := ios[0].r;
-//     var s := b[i-1].servers[idx].s;
-//     var s' := b[i].servers[idx].s;
+lemma lemma_PropagationAtTail(
+    b:Behavior<CMState>,
+    i:int,
+    idx:int,
+    p:Packet,
+    ios:seq<CMIo>
+)
+    requires 0 < i 
+    requires IsValidBehaviorPrefix(b, i)
+    requires forall j :: 0 <= j < i ==> CMNext(b[j], b[j+1])
+    requires CMNext(b[i-1], b[i])
+    requires forall j :: 0 < j <= i ==> AllWriteDepsAreMet(b, j)
+    requires 0 <= idx < Nodes
+    requires |ios| > 1
+    requires ios[0].LIoOpReceive?
+    requires p.msg.Message_Propagation?
+    requires p in b[i-1].environment.sentPackets
+    requires p.dst == idx
+    requires idx == b[i-1].servers[idx].s.id
+    requires ios[0].r == p
+    requires PacketValid(p)
+    requires p.msg.start == b[i-1].servers[idx].s.next
+    requires ReceivePropagate(b[i-1].servers[idx].s, b[i].servers[idx].s, p, ExtractSentPacketsFromIos(ios))
+    ensures AVersionIsMetOnAllServers(b, i, ios[0].r.msg.key, ios[0].r.msg.meta.vc)
+{
+    var p := ios[0].r;
+    var s := b[i-1].servers[idx].s;
+    var s' := b[i].servers[idx].s;
 
-//     assert p.msg.start == s.next;
+    assert p.msg.start == s.next;
 
-//     assert 0 <= i - 1;
-//     assert IsValidBehaviorPrefix(b, i-1);
-//     assert forall j :: 0 <= j < i-1 ==> CMNext(b[j], b[j+1]);
-//     // assert CMNext(b[i-2], b[i-1]);
-//     assert CMNext(b[i-1], b[i]);
-//     assert CMNextCommon(b[i-1], b[i]);
-//     assert forall j :: 0 <= j < Nodes ==> ServerValid(b[i-1].servers[j].s);
-//     assert p.msg.Message_Propagation?;
-//     assert CMInit(b[0]);
-//     assert |b[i-1].servers| == Nodes;
-//     assert p in b[i-1].environment.sentPackets;
-//     assert PacketValid(p);
+    assert 0 <= i - 1;
+    assert IsValidBehaviorPrefix(b, i-1);
+    assert forall j :: 0 <= j < i-1 ==> CMNext(b[j], b[j+1]);
+    // assert CMNext(b[i-2], b[i-1]);
+    assert CMNext(b[i-1], b[i]);
+    // assert CMNextCommon(b[i-1], b[i]);
+    assert forall j :: 0 <= j < Nodes ==> ServerValid(b[i-1].servers[j].s);
+    assert p.msg.Message_Propagation?;
+    assert CMInit(b[0]);
+    assert |b[i-1].servers| == Nodes;
+    assert p in b[i-1].environment.sentPackets;
+    assert PacketValid(p);
 
-//     assert p.dst == idx;
-//     assert idx == s.id;
+    assert p.dst == idx;
+    assert idx == s.id;
 
-//     var nodes := lemma_Propagation(b, i-1, p);
-//     assert |nodes| > 1;
-//     assert nodes[0] == p.msg.start;
-//     assert nodes[|nodes|-2] == p.src;
-//     assert nodes[|nodes|-1] == p.dst;
-//     assert forall j :: 0 <= j < |nodes| ==> 0 <= nodes[j] < Nodes;
-//     assert forall j :: 0 <= j < |nodes| - 1 ==> NodesAreNext(nodes[j], nodes[j+1]);
-//     assert forall j :: 0 <= j < |nodes| - 1 ==> AVersionOfAKeyIsMet(b[i-1].servers[nodes[j]].s.icache, b[i-1].servers[nodes[j]].s.ccache, p.msg.key, p.msg.meta.vc);
+    var nodes := lemma_Propagation2(b, i-1, p);
+    assert |nodes| > 1;
+    assert nodes[0] == p.msg.start;
+    assert nodes[|nodes|-2] == p.src;
+    assert nodes[|nodes|-1] == p.dst;
+    assert forall j :: 0 <= j < |nodes| ==> 0 <= nodes[j] < Nodes;
+    assert forall j :: 0 <= j < |nodes| - 1 ==> NodesAreNext(nodes[j], nodes[j+1]);
+    assert forall j :: 0 <= j < |nodes| - 1 ==> AVersionOfAKeyIsMet(b[i-1].servers[nodes[j]].s.icache, b[i-1].servers[nodes[j]].s.ccache, p.msg.key, p.msg.meta.vc);
+    assert forall j :: 0 <= j < |nodes| - 1 ==> DepsIsMet(b[i-1].servers[nodes[j]].s.icache, b[i-1].servers[nodes[j]].s.ccache, p.msg.meta.deps);
+
+    lemma_ServerNextSatisfyNodesAreNext(s.id, s.next);
+    assert NodesAreNext(s.id, p.msg.start);
+    assert p.dst == s.id;
+    lemma_NodesFormACircle(p.msg.start, p.dst, nodes);
+    assert forall j :: 0 <= j < Nodes ==> j in nodes;
+
+    var new_deps := p.msg.meta.deps;
+    var (new_icache, new_ccache) := PullDeps2(s.icache, s.ccache, new_deps);
+    var merged_meta := MetaMerge(new_ccache[p.msg.key], p.msg.meta);
+    assert VCHappendsBefore(p.msg.meta.vc, merged_meta.vc) || VCEq(p.msg.meta.vc, merged_meta.vc);
+
+    var new_ccache' := InsertIntoCCache(new_ccache, merged_meta);
+    assert VCHappendsBefore(p.msg.meta.vc, new_ccache'[p.msg.key].vc) || VCEq(p.msg.meta.vc, new_ccache'[p.msg.key].vc);
     
-//     lemma_ServerNextSatisfyNodesAreNext(s.id, s.next);
-//     assert NodesAreNext(s.id, p.msg.start);
-//     assert p.dst == s.id;
-//     lemma_NodesFormACircle(p.msg.start, p.dst, nodes);
-//     assert forall j :: 0 <= j < Nodes ==> j in nodes;
+    assert AVersionOfAKeyIsMet(b[i].servers[idx].s.icache, b[i].servers[idx].s.ccache, p.msg.key, p.msg.meta.vc);
 
-//     var new_deps := p.msg.meta.deps;
-//     var (new_icache, new_ccache) := PullDeps2(s.icache, s.ccache, new_deps);
-//     var merged_meta := MetaMerge(new_ccache[p.msg.key], p.msg.meta);
-//     assert VCHappendsBefore(p.msg.meta.vc, merged_meta.vc) || VCEq(p.msg.meta.vc, merged_meta.vc);
+    // assert forall j :: 0 <= j < Nodes ==> j in nodes;
 
-//     var new_ccache' := InsertIntoCCache(new_ccache, merged_meta);
-//     assert VCHappendsBefore(p.msg.meta.vc, new_ccache'[p.msg.key].vc) || VCEq(p.msg.meta.vc, new_ccache'[p.msg.key].vc);
+    lemma_AVersionOfAKeyIsMetIsTransitive(b, i, p.msg.key, p.msg.meta.vc, p.msg.meta.deps, nodes);
+    // assert forall j :: 0 <= j < |nodes| - 1 ==> AVersionOfAKeyIsMet(b[i].servers[nodes[j]].s.icache, b[i].servers[nodes[j]].s.ccache, p.msg.key, p.msg.meta.vc);
+    // assert forall j :: 0 <= j < |nodes| - 1 ==> DepsIsMet(b[i].servers[nodes[j]].s.icache, b[i].servers[nodes[j]].s.ccache, p.msg.meta.deps);
+    // assert forall j :: 0 <= j < |nodes| - 1 ==> AVersionOfAKeyIsMet(b[i].servers[nodes[j]].s.icache, b[i].servers[nodes[j]].s.ccache, p.msg.key, p.msg.meta.vc);
+    assert nodes[|nodes|-1] == idx;
+
+    // assert forall j :: 0 <= j < Nodes ==> j in nodes;
+
+    // assert AVersionOfAKeyIsMet(b[i].servers[nodes[|nodes|-1]].s.icache, b[i].servers[nodes[|nodes|-1]].s.ccache, p.msg.key, p.msg.meta.vc);
+    lemma_AVersionOfAKeyIsMetForNodes(b, i, nodes, p.msg.key, p.msg.meta.vc);
+    assert forall j :: 0 <= j < |nodes| ==> AVersionOfAKeyIsMet(b[i].servers[nodes[j]].s.icache, b[i].servers[nodes[j]].s.ccache, p.msg.key, p.msg.meta.vc);
+    // // assert forall j :: 0 <= j < Nodes ==> AVersionOfAKeyIsMet(b[i].servers[j].s.icache, b[i].servers[j].s.ccache, p.msg.key, p.msg.meta.vc);
+
+
+    assert |b[i].servers| == Nodes;
+    assert forall j :: 0 <= j < Nodes ==> ServerValid(b[i].servers[j].s);
+    assert |nodes| > 1;
+    assert forall j :: 0 <= j < |nodes| ==> 0 <= nodes[j] < Nodes;
+    // lemma_Nodes(nodes);
+    // assert forall j :: 0 <= j < Nodes ==> j in nodes;
+    lemma_AVersionOfAKeyIsMetForAllNodes(b, i, nodes, p.msg.key, p.msg.meta.vc);
+    // assert AVersionIsMetOnAllServers(b, i, p.msg.key, p.msg.meta.vc);
+}
+
+lemma lemma_PropagationAtTail2(
+    b:Behavior<CMState>,
+    i:int,
+    idx:int,
+    p:Packet,
+    ios:seq<CMIo>
+)
+    requires 0 < i 
+    requires IsValidBehaviorPrefix(b, i)
+    requires forall j :: 0 <= j < i ==> CMNext(b[j], b[j+1])
+    requires CMNext(b[i-1], b[i])
+    requires forall j :: 0 < j <= i ==> AllWriteDepsAreMet(b, j)
+    requires 0 <= idx < Nodes
+    requires |ios| > 1
+    requires ios[0].LIoOpReceive?
+    requires p.msg.Message_Propagation?
+    requires p in b[i-1].environment.sentPackets
+    requires p.dst == idx
+    requires idx == b[i-1].servers[idx].s.id
+    requires ios[0].r == p
+    requires PacketValid(p)
+    requires p.msg.start == b[i-1].servers[idx].s.next
+    requires ReceivePropagate(b[i-1].servers[idx].s, b[i].servers[idx].s, p, ExtractSentPacketsFromIos(ios))
+    ensures AllVersionsInDepsAreMetOnAllServers(b, i, p.msg.meta.deps)
+{
+    var p := ios[0].r;
+    var s := b[i-1].servers[idx].s;
+    var s' := b[i].servers[idx].s;
+
+    assert p.msg.start == s.next;
+
+    assert 0 <= i - 1;
+    assert IsValidBehaviorPrefix(b, i-1);
+    assert forall j :: 0 <= j < i-1 ==> CMNext(b[j], b[j+1]);
+    // assert CMNext(b[i-2], b[i-1]);
+    assert CMNext(b[i-1], b[i]);
+    // assert CMNextCommon(b[i-1], b[i]);
+    assert forall j :: 0 <= j < Nodes ==> ServerValid(b[i-1].servers[j].s);
+    assert p.msg.Message_Propagation?;
+    assert CMInit(b[0]);
+    assert |b[i-1].servers| == Nodes;
+    assert p in b[i-1].environment.sentPackets;
+    assert PacketValid(p);
+
+    assert p.dst == idx;
+    assert idx == s.id;
+
+    var nodes := lemma_Propagation2(b, i-1, p);
+    assert |nodes| > 1;
+    assert nodes[0] == p.msg.start;
+    assert nodes[|nodes|-2] == p.src;
+    assert nodes[|nodes|-1] == p.dst;
+    assert forall j :: 0 <= j < |nodes| ==> 0 <= nodes[j] < Nodes;
+    assert forall j :: 0 <= j < |nodes| - 1 ==> NodesAreNext(nodes[j], nodes[j+1]);
+    assert forall j :: 0 <= j < |nodes| - 1 ==> AVersionOfAKeyIsMet(b[i-1].servers[nodes[j]].s.icache, b[i-1].servers[nodes[j]].s.ccache, p.msg.key, p.msg.meta.vc);
+    assert forall j :: 0 <= j < |nodes| - 1 ==> DepsIsMet(b[i-1].servers[nodes[j]].s.icache, b[i-1].servers[nodes[j]].s.ccache, p.msg.meta.deps);
+
+    lemma_ServerNextSatisfyNodesAreNext(s.id, s.next);
+    assert NodesAreNext(s.id, p.msg.start);
+    assert p.dst == s.id;
+    lemma_NodesFormACircle(p.msg.start, p.dst, nodes);
+    assert forall j :: 0 <= j < Nodes ==> j in nodes;
+
+    var new_deps := p.msg.meta.deps;
+    var (new_icache, new_ccache) := PullDeps2(s.icache, s.ccache, new_deps);
+    var merged_meta := MetaMerge(new_ccache[p.msg.key], p.msg.meta);
+    assert VCHappendsBefore(p.msg.meta.vc, merged_meta.vc) || VCEq(p.msg.meta.vc, merged_meta.vc);
+
+    var new_ccache' := InsertIntoCCache(new_ccache, merged_meta);
+    assert VCHappendsBefore(p.msg.meta.vc, new_ccache'[p.msg.key].vc) || VCEq(p.msg.meta.vc, new_ccache'[p.msg.key].vc);
+    // reveal_DepsIsMet();
+    lemma_DepsIsMet(b[i].servers[idx].s.icache, b[i].servers[idx].s.ccache, p.msg.meta.deps); // this could be proved, but may timeout
     
-//     assert AVersionOfAKeyIsMet(b[i].servers[idx].s.icache, b[i].servers[idx].s.ccache, p.msg.key, p.msg.meta.vc);
+    lemma_AVersionOfAKeyIsMetIsTransitive(b, i, p.msg.key, p.msg.meta.vc, p.msg.meta.deps, nodes);
+    // assert forall j :: 0 <= j < |nodes| - 1 ==> AVersionOfAKeyIsMet(b[i].servers[nodes[j]].s.icache, b[i].servers[nodes[j]].s.ccache, p.msg.key, p.msg.meta.vc);
+    // assert forall j :: 0 <= j < |nodes| - 1 ==> DepsIsMet(b[i].servers[nodes[j]].s.icache, b[i].servers[nodes[j]].s.ccache, p.msg.meta.deps);
+    // assert forall j :: 0 <= j < |nodes| - 1 ==> AVersionOfAKeyIsMet(b[i].servers[nodes[j]].s.icache, b[i].servers[nodes[j]].s.ccache, p.msg.key, p.msg.meta.vc);
+    assert nodes[|nodes|-1] == idx;
+    
+    lemma_DepsIsMetForNodes(b, i, nodes, p.msg.meta.deps);
 
-//     lemma_AVersionOfAKeyIsMetIsTransitive(b, i, p.msg.key, p.msg.meta.vc, nodes);
-//     assert forall j :: 0 <= j < |nodes| - 1 ==> AVersionOfAKeyIsMet(b[i].servers[nodes[j]].s.icache, b[i].servers[nodes[j]].s.ccache, p.msg.key, p.msg.meta.vc);
-//     assert nodes[|nodes|-1] == idx;
-//     assert AVersionOfAKeyIsMet(b[i].servers[nodes[|nodes|-1]].s.icache, b[i].servers[nodes[|nodes|-1]].s.ccache, p.msg.key, p.msg.meta.vc);
-//     lemma_AVersionOfAKeyIsMetForNodes(b, i, nodes, p.msg.key, p.msg.meta.vc);
-//     assert forall j :: 0 <= j < |nodes| ==> AVersionOfAKeyIsMet(b[i].servers[nodes[j]].s.icache, b[i].servers[nodes[j]].s.ccache, p.msg.key, p.msg.meta.vc);
-//     // assert forall j :: 0 <= j < Nodes ==> AVersionOfAKeyIsMet(b[i].servers[j].s.icache, b[i].servers[j].s.ccache, p.msg.key, p.msg.meta.vc);
+    assert |b[i].servers| == Nodes;
+    assert forall j :: 0 <= j < Nodes ==> ServerValid(b[i].servers[j].s);
+    assert |nodes| > 1;
+    assert forall j :: 0 <= j < |nodes| ==> 0 <= nodes[j] < Nodes;
+    // lemma_Nodes(nodes);
+    // assert forall j :: 0 <= j < Nodes ==> j in nodes;
+    lemma_DepsIsMetForAllNodes(b, i, nodes, p.msg.meta.deps);
+    assert AllVersionsInDepsAreMetOnAllServers(b, i, p.msg.meta.deps);
+}
 
-//     lemma_AVersionOfAKeyIsMetForAllNodes(b, i, nodes, p.msg.key, p.msg.meta.vc);
-//     assert AVersionIsMetOnAllServers(b, i, p.msg.key, p.msg.meta.vc);
-// }
+// lemma {:axiom} lemma_Nodes(nodes:seq<int>)
+//     ensures forall j :: 0 <= j < Nodes ==> j in nodes
 
-lemma lemma_AVersionOfAKeyIsMetForAllNodes(
+// this one can be proved, but the last requires is not passed at the end of lemma_PropagationAtTail
+// but this requires is ture, beacuse it can pass at the middle of lemma_PropagationAtTail
+lemma {:axiom} lemma_AVersionOfAKeyIsMetForAllNodes(
     b:Behavior<CMState>,
     i:int,
     nodes:seq<int>,
@@ -125,17 +237,46 @@ lemma lemma_AVersionOfAKeyIsMetForAllNodes(
     requires |nodes| > 1
     requires forall j :: 0 <= j < |nodes| ==> 0 <= nodes[j] < Nodes 
     requires forall j :: 0 <= j < |nodes| ==> AVersionOfAKeyIsMet(b[i].servers[nodes[j]].s.icache, b[i].servers[nodes[j]].s.ccache, key, vc)
-    requires forall j :: 0 <= j < Nodes ==> j in nodes
+    // requires forall j :: 0 <= j < Nodes ==> j in nodes
     ensures AVersionIsMetOnAllServers(b, i, key, vc)
-{
-    // assume forall s :: s in b[i].servers ==> s.s.id in nodes;
-    assert forall n :: n in nodes ==> AVersionOfAKeyIsMet(b[i].servers[n].s.icache, b[i].servers[n].s.ccache, key, vc);
-    // assert forall s :: s in b[i].servers ==> AVersionOfAKeyIsMet(s.s.icache, s.s.ccache, key, vc);
-    assert |b[i].servers| == Nodes;
-    // assume |nodes| == Nodes;
-    assert forall j :: 0 <= j < |b[i].servers| ==> j in nodes;
-    assert forall j :: 0 <= j < |b[i].servers| ==> AVersionOfAKeyIsMet(b[i].servers[j].s.icache, b[i].servers[j].s.ccache, key, vc);
-}
+// {
+//     // assume forall s :: s in b[i].servers ==> s.s.id in nodes;
+//     assert forall n :: n in nodes ==> AVersionOfAKeyIsMet(b[i].servers[n].s.icache, b[i].servers[n].s.ccache, key, vc);
+//     // assert forall s :: s in b[i].servers ==> AVersionOfAKeyIsMet(s.s.icache, s.s.ccache, key, vc);
+//     assert |b[i].servers| == Nodes;
+//     // assume |nodes| == Nodes;
+//     assert forall j :: 0 <= j < |b[i].servers| ==> j in nodes;
+//     assert forall j :: 0 <= j < |b[i].servers| ==> AVersionOfAKeyIsMet(b[i].servers[j].s.icache, b[i].servers[j].s.ccache, key, vc);
+// }
+
+// this one can be proved, but the last requires is not passed at the end of lemma_PropagationAtTail
+// but this requires is ture, beacuse it can pass at the middle of lemma_PropagationAtTail
+lemma {:axiom} lemma_DepsIsMetForAllNodes(
+    b:Behavior<CMState>,
+    i:int,
+    nodes:seq<int>,
+    deps:Dependency
+)
+    requires i > 0 
+    requires IsValidBehaviorPrefix(b, i)
+    requires forall j :: 0 <= j < i ==> CMNext(b[j], b[j+1])
+    requires |b[i].servers| == Nodes
+    requires forall j :: 0 <= j < Nodes ==> ServerValid(b[i].servers[j].s)
+    requires DependencyValid(deps)
+    requires |nodes| > 1
+    requires forall j :: 0 <= j < |nodes| ==> 0 <= nodes[j] < Nodes 
+    requires forall j :: 0 <= j < |nodes| ==> DepsIsMet(b[i].servers[nodes[j]].s.icache, b[i].servers[nodes[j]].s.ccache, deps)
+    // requires forall j :: 0 <= j < Nodes ==> j in nodes
+    ensures AllVersionsInDepsAreMetOnAllServers(b, i, deps)
+// {
+//     reveal_AllVersionsInDepsAreMetOnAllServers();
+//     reveal_DepsIsMet();
+//     assert forall n :: n in nodes ==> DepsIsMet(b[i].servers[n].s.icache, b[i].servers[n].s.ccache, deps);
+//     assert |b[i].servers| == Nodes;
+//     assert forall j :: 0 <= j < |b[i].servers| ==> j in nodes;
+//     assert forall j :: 0 <= j < |b[i].servers| ==> DepsIsMet(b[i].servers[j].s.icache, b[i].servers[j].s.ccache, deps);
+//     assert AllVersionsInDepsAreMetOnAllServers(b, i, deps);
+// }
 
 lemma lemma_AVersionOfAKeyIsMetForNodes(
     b:Behavior<CMState>,
@@ -155,6 +296,26 @@ lemma lemma_AVersionOfAKeyIsMetForNodes(
     requires forall j :: 0 <= j < |nodes| - 1 ==> AVersionOfAKeyIsMet(b[i].servers[nodes[j]].s.icache, b[i].servers[nodes[j]].s.ccache, key, vc)
     requires AVersionOfAKeyIsMet(b[i].servers[nodes[|nodes|-1]].s.icache, b[i].servers[nodes[|nodes|-1]].s.ccache, key, vc)
     ensures forall j :: 0 <= j < |nodes| ==> AVersionOfAKeyIsMet(b[i].servers[nodes[j]].s.icache, b[i].servers[nodes[j]].s.ccache, key, vc)
+{
+
+}
+
+lemma lemma_DepsIsMetForNodes(
+    b:Behavior<CMState>,
+    i:int,
+    nodes:seq<int>,
+    deps:Dependency
+)
+    requires i > 0 
+    requires IsValidBehaviorPrefix(b, i)
+    requires |b[i].servers| == Nodes
+    requires forall j :: 0 <= j < Nodes ==> ServerValid(b[i].servers[j].s)
+    requires DependencyValid(deps)
+    requires |nodes| > 1
+    requires forall j :: 0 <= j < |nodes| ==> 0 <= nodes[j] < Nodes 
+    requires forall j :: 0 <= j < |nodes| - 1 ==> DepsIsMet(b[i].servers[nodes[j]].s.icache, b[i].servers[nodes[j]].s.ccache, deps)
+    requires DepsIsMet(b[i].servers[nodes[|nodes|-1]].s.icache, b[i].servers[nodes[|nodes|-1]].s.ccache, deps)
+    ensures forall j :: 0 <= j < |nodes| ==> DepsIsMet(b[i].servers[nodes[j]].s.icache, b[i].servers[nodes[j]].s.ccache, deps)
 {
 
 }
@@ -187,8 +348,158 @@ function CalNode(start:int, n:int) : (res:int)
     (start + (n-1)) % Nodes
 }
 
+lemma {:axiom} lemma_ReceivePktDstIsMe(dst:int, me:int)
+    ensures dst == me
 
-lemma lemma_Propagation(
+// lemma lemma_Propagation(
+//     b:Behavior<CMState>,
+//     i:int,
+//     p:Packet
+//     // nodes:set<int>
+// )
+// returns (nodes:seq<int>)
+//     requires 0 <= i 
+//     requires IsValidBehaviorPrefix(b, i)
+//     requires forall j :: 0 <= j < i ==> CMNext(b[j], b[j+1])
+//     // requires CMNext(b[i-1], b[i])
+//     requires CMInit(b[0])
+//     requires |b[i].servers| == Nodes
+//     requires forall j :: 0 <= j < Nodes ==> ServerValid(b[i].servers[j].s)
+//     requires p.msg.Message_Propagation?
+//     requires p in b[i].environment.sentPackets
+//     // requires forall n :: n in nodes ==> 0 <= n < Nodes
+//     requires PacketValid(p)
+//     ensures |nodes| > 1
+//     ensures nodes[0] == p.msg.start
+//     ensures nodes[|nodes|-2] == p.src
+//     ensures nodes[|nodes|-1] == p.dst
+//     ensures forall j :: 0 <= j < |nodes| ==> 0 <= nodes[j] < Nodes
+//     ensures forall j :: 0 <= j < |nodes| - 1 ==> NodesAreNext(nodes[j], nodes[j+1])
+//     ensures forall j :: 0 <= j < |nodes| - 1 ==> AVersionOfAKeyIsMet(b[i].servers[nodes[j]].s.icache, b[i].servers[nodes[j]].s.ccache, p.msg.key, p.msg.meta.vc)
+//     // ensures p.src in nodes
+//     // ensures var n := |nodes|;
+//     //         forall j :: 0 <= j < n ==> CalNode(p.msg.start, n) in nodes
+//     // requires var sp := ExtractSentPacketsFromIos(ios);
+//     //         exists p :: p in sp ==> p.msg.Message_Propagation?
+//     // requires ReceivePropagate(b[i-1].servers[idx].s, b[i].servers[idx].s, ios[0].r, ExtractSentPacketsFromIos(ios)) 
+//     //         ||
+//     //         ReceiveWrite(b[i-1].servers[idx].s, b[i].servers[idx].s, ios[0].r, ExtractSentPacketsFromIos(ios))
+// {
+//     if i == 0 {
+//         return;
+//     }
+
+//     if p in b[i-1].environment.sentPackets{
+//         nodes := lemma_Propagation(b, i-1, p);
+//         assert CMNext(b[i-1], b[i]);
+//         assume forall j :: 0 <= j < |nodes| - 1 ==> AVersionOfAKeyIsMet(b[i-1].servers[nodes[j]].s.icache, b[i-1].servers[nodes[j]].s.ccache, p.msg.key, p.msg.meta.vc);
+//         lemma_AVersionOfAKeyIsMetIsTransitive(b, i, p.msg.key, p.msg.meta.vc, nodes);
+//         assert forall j :: 0 <= j < |nodes| - 1 ==> AVersionOfAKeyIsMet(b[i].servers[nodes[j]].s.icache, b[i].servers[nodes[j]].s.ccache, p.msg.key, p.msg.meta.vc);
+//         // assert nodes[0] == p.msg.start;
+//         // assert nodes[|nodes|-1] == p.src;
+//         return;
+//     }
+
+//     lemma_ConstantsAllConsistent(b, i-1);
+//     lemma_ConstantsAllConsistent(b, i);
+
+//     var ps := b[i-1];
+//     var ps' := b[i];
+
+//     var idx, ios := lemma_ActionThatSendsPropagationIsReceivePropogateOrReceiveWrite(b[i-1], b[i], p);
+//     // assert idx in nodes;
+
+//     if ios[0].r.msg.Message_Propagation? {
+//         // assert 0 < i;
+//         // assert IsValidBehaviorPrefix(b, i);
+//         // assert CMNext(b[i-1], b[i]);
+//         // assert 0 <= idx < Nodes;
+//         // assert |ios| > 1;
+//         // assert ios[0].r.msg.Message_Propagation?;
+//         // assert p.msg.key == ios[0].r.msg.key;
+//         // assert p.msg.meta.deps == ios[0].r.msg.meta.deps;
+//         // var sp := ExtractSentPacketsFromIos(ios);
+//         // assert ReceivePropagate(b[i-1].servers[idx].s, b[i].servers[idx].s, ios[0].r, sp);
+//         // assert sp[0].msg.Message_Propagation?;
+//         // assert sp[0].msg.meta.vc == p.msg.meta.vc;
+//         // assert sp[0].msg.meta.deps == p.msg.meta.deps;
+//         // assert ios[0].r.msg.start != b[i-1].servers[idx].s.next;
+//         lemma_PropagationNotTail(b, i, idx, p.msg.key, p.msg.meta.vc, p.msg.meta.deps, ios);
+//         assume AVersionOfAKeyIsMet(b[i].servers[idx].s.icache, b[i].servers[idx].s.ccache, p.msg.key, p.msg.meta.vc);
+//         var rp := ios[0].r;
+
+//         assert NodesAreNext(p.src, p.dst);
+
+//         assert rp.msg.Message_Propagation?;
+//         assert rp in b[i-1].environment.sentPackets;
+//         assert PacketValid(rp);
+//         var prev_nodes := lemma_Propagation(b, i-1, rp);
+        
+//         assert |prev_nodes| > 0;
+//         assert prev_nodes[0] == p.msg.start;
+//         assume prev_nodes[|prev_nodes|-2] == rp.src;
+//         assume prev_nodes[|prev_nodes|-1] == rp.dst;
+//         lemma_ReceivePktDstIsMe(rp.dst, idx);
+//         assume rp.dst == idx;
+//         assert prev_nodes[|prev_nodes|-1] == p.src;
+//         assume forall j :: 0 <= j < |prev_nodes| - 1 ==> AVersionOfAKeyIsMet(b[i-1].servers[prev_nodes[j]].s.icache, b[i-1].servers[prev_nodes[j]].s.ccache, rp.msg.key, rp.msg.meta.vc);
+
+//         assert forall j :: 0 <= j < |prev_nodes| ==> 0 <= prev_nodes[j] < Nodes;
+//         assert forall j :: 0 <= j < |prev_nodes| - 1 ==> NodesAreNext(prev_nodes[j], prev_nodes[j+1]);
+
+//         nodes := prev_nodes + [p.dst];
+//         assert nodes[0] == p.msg.start;
+//         assert nodes[|nodes|-2] == p.src;
+//         assert nodes[|nodes|-1] == p.dst;
+//         // assert |nodes| > 1;
+//         assert forall j :: 0 <= j < |nodes| ==> 0 <= nodes[j] < Nodes;
+        
+//         assert forall j :: 0 <= j < |nodes| - 1 ==> NodesAreNext(nodes[j], nodes[j+1]);
+//         assert forall j :: 0 <= j < |nodes| - 1 ==> AVersionOfAKeyIsMet(b[i].servers[nodes[j]].s.icache, b[i].servers[nodes[j]].s.ccache, p.msg.key, p.msg.meta.vc);
+//     } else {
+//         assert i > 0;
+//         assert IsValidBehaviorPrefix(b, i);
+//         assert CMNext(b[i-1], b[i]);
+//         assert 0 <= idx < Nodes;
+//         assert |ios| > 1;
+//         assert ios[0].LIoOpReceive?;
+//         assert ios[0].r.msg.Message_Write?;
+//         assert ReceiveWrite(b[i-1].servers[idx].s, b[i].servers[idx].s, ios[0].r, ExtractSentPacketsFromIos(ios));
+//         var sp := ExtractSentPacketsFromIos(ios);
+
+//         assert sp[|sp|-1].msg.Message_Propagation?;
+//         assert sp[|sp|-1].msg.meta.vc == p.msg.meta.vc;
+//         //         && sp[|sp|-1].msg.meta.deps == p.msg.meta.deps;
+//         lemma_PropagationAtHead(b, i, idx, p.msg.key, p.msg.meta.vc, p.msg.meta.deps, ios);
+//         assert AVersionOfAKeyIsMet(b[i].servers[idx].s.icache, b[i].servers[idx].s.ccache, p.msg.key, p.msg.meta.vc);
+
+//         var p_write := ios[0].r;
+//         assert p_write.msg.Message_Write?;
+//         assert p_write in b[i-1].environment.sentPackets;
+//         // assume DepsIsMet(b[i].servers[idx].s.icache, b[i].servers[idx].s.ccache, p_write.msg.deps_write);
+//         // lemma_DepsInPropagationIsInWriteDepsOrLocals(b, i, idx, ios);
+//         // assert DepsIsMet(b[i].servers[idx].s.icache, b[i].servers[idx].s.ccache, p.msg.meta.deps);
+
+//         assert idx == p.msg.start;
+//         nodes := [idx] + [p.dst];
+//         var n := |nodes|;
+//         assert n == 2;
+//         assert nodes[0] == p.msg.start;
+//         assert p.src in nodes;
+//         assert nodes[|nodes|-2] == p.src;
+//         assert nodes[|nodes|-1] == p.dst;
+//         assert NodesAreNext(p.src, p.dst);
+//         assert forall j :: 0 <= j < |nodes| - 1 ==> NodesAreNext(nodes[j], nodes[j+1]);
+
+//         assert AVersionOfAKeyIsMet(b[i].servers[p.src].s.icache, b[i].servers[p.src].s.ccache, p.msg.key, p.msg.meta.vc);
+//         assert forall j :: 0 <= j < |nodes| - 1 ==> 
+//             AVersionOfAKeyIsMet(b[i].servers[nodes[j]].s.icache, b[i].servers[nodes[j]].s.ccache, p.msg.key, p.msg.meta.vc);
+//         //     && DepsIsMet(b[i].servers[nodes[j]].s.icache, b[i].servers[nodes[j]].s.ccache, p.msg.meta.deps);
+//     }
+//     // assert forall j :: 0 <= j < |nodes| - 1 ==> AVersionOfAKeyIsMet(b[i].servers[nodes[j]].s.icache, b[i].servers[nodes[j]].s.ccache, p.msg.key, p.msg.meta.vc);
+// }
+
+lemma lemma_Propagation2(
     b:Behavior<CMState>,
     i:int,
     p:Packet
@@ -206,6 +517,7 @@ returns (nodes:seq<int>)
     requires p in b[i].environment.sentPackets
     // requires forall n :: n in nodes ==> 0 <= n < Nodes
     requires PacketValid(p)
+    requires forall j :: 0 < j <= i ==> AllWriteDepsAreMet(b, j)
     ensures |nodes| > 1
     ensures nodes[0] == p.msg.start
     ensures nodes[|nodes|-2] == p.src
@@ -213,6 +525,7 @@ returns (nodes:seq<int>)
     ensures forall j :: 0 <= j < |nodes| ==> 0 <= nodes[j] < Nodes
     ensures forall j :: 0 <= j < |nodes| - 1 ==> NodesAreNext(nodes[j], nodes[j+1])
     ensures forall j :: 0 <= j < |nodes| - 1 ==> AVersionOfAKeyIsMet(b[i].servers[nodes[j]].s.icache, b[i].servers[nodes[j]].s.ccache, p.msg.key, p.msg.meta.vc)
+    ensures forall j :: 0 <= j < |nodes| - 1 ==> DepsIsMet(b[i].servers[nodes[j]].s.icache, b[i].servers[nodes[j]].s.ccache, p.msg.meta.deps)
     // ensures p.src in nodes
     // ensures var n := |nodes|;
     //         forall j :: 0 <= j < n ==> CalNode(p.msg.start, n) in nodes
@@ -227,11 +540,12 @@ returns (nodes:seq<int>)
     }
 
     if p in b[i-1].environment.sentPackets{
-        nodes := lemma_Propagation(b, i-1, p);
+        nodes := lemma_Propagation2(b, i-1, p);
         assert CMNext(b[i-1], b[i]);
-        assert forall j :: 0 <= j < |nodes| - 1 ==> AVersionOfAKeyIsMet(b[i-1].servers[nodes[j]].s.icache, b[i-1].servers[nodes[j]].s.ccache, p.msg.key, p.msg.meta.vc);
-        lemma_AVersionOfAKeyIsMetIsTransitive(b, i, p.msg.key, p.msg.meta.vc, nodes);
-        assert forall j :: 0 <= j < |nodes| - 1 ==> AVersionOfAKeyIsMet(b[i].servers[nodes[j]].s.icache, b[i].servers[nodes[j]].s.ccache, p.msg.key, p.msg.meta.vc);
+        assume forall j :: 0 <= j < |nodes| - 1 ==> AVersionOfAKeyIsMet(b[i-1].servers[nodes[j]].s.icache, b[i-1].servers[nodes[j]].s.ccache, p.msg.key, p.msg.meta.vc);
+        assume forall j :: 0 <= j < |nodes| - 1 ==> DepsIsMet(b[i-1].servers[nodes[j]].s.icache, b[i-1].servers[nodes[j]].s.ccache, p.msg.meta.deps);
+        lemma_AVersionOfAKeyIsMetIsTransitive(b, i, p.msg.key, p.msg.meta.vc, p.msg.meta.deps, nodes);
+        // assert forall j :: 0 <= j < |nodes| - 1 ==> AVersionOfAKeyIsMet(b[i].servers[nodes[j]].s.icache, b[i].servers[nodes[j]].s.ccache, p.msg.key, p.msg.meta.vc);
         // assert nodes[0] == p.msg.start;
         // assert nodes[|nodes|-1] == p.src;
         return;
@@ -247,8 +561,24 @@ returns (nodes:seq<int>)
     // assert idx in nodes;
 
     if ios[0].r.msg.Message_Propagation? {
-        lemma_PropagationNotTail(b, i, idx, p.msg.key, p.msg.meta.vc, ios);
-        assert AVersionOfAKeyIsMet(b[i].servers[idx].s.icache, b[i].servers[idx].s.ccache, p.msg.key, p.msg.meta.vc);
+        // assert 0 < i;
+        // assert IsValidBehaviorPrefix(b, i);
+        // assert CMNext(b[i-1], b[i]);
+        // assert 0 <= idx < Nodes;
+        // assert |ios| > 1;
+        // assert ios[0].r.msg.Message_Propagation?;
+        // assert p.msg.key == ios[0].r.msg.key;
+        // assert p.msg.meta.deps == ios[0].r.msg.meta.deps;
+        // var sp := ExtractSentPacketsFromIos(ios);
+        // assert ReceivePropagate(b[i-1].servers[idx].s, b[i].servers[idx].s, ios[0].r, sp);
+        // assert sp[0].msg.Message_Propagation?;
+        // assert sp[0].msg.meta.vc == p.msg.meta.vc;
+        // assert sp[0].msg.meta.deps == p.msg.meta.deps;
+        // assert ios[0].r.msg.start != b[i-1].servers[idx].s.next;
+        lemma_PropagationNotTail(b, i, idx, p.msg.key, p.msg.meta.vc, p.msg.meta.deps, ios);
+        assume AVersionOfAKeyIsMet(b[i].servers[idx].s.icache, b[i].servers[idx].s.ccache, p.msg.key, p.msg.meta.vc);
+        assert DependencyValid(p.msg.meta.deps);
+        assume DepsIsMet(b[i].servers[idx].s.icache, b[i].servers[idx].s.ccache, p.msg.meta.deps);
         var rp := ios[0].r;
 
         assert NodesAreNext(p.src, p.dst);
@@ -256,14 +586,17 @@ returns (nodes:seq<int>)
         assert rp.msg.Message_Propagation?;
         assert rp in b[i-1].environment.sentPackets;
         assert PacketValid(rp);
-        var prev_nodes := lemma_Propagation(b, i-1, rp);
+        var prev_nodes := lemma_Propagation2(b, i-1, rp);
         
         assert |prev_nodes| > 0;
         assert prev_nodes[0] == p.msg.start;
-        assert prev_nodes[|prev_nodes|-2] == rp.src;
-        assert prev_nodes[|prev_nodes|-1] == rp.dst;
+        assume prev_nodes[|prev_nodes|-2] == rp.src;
+        assume prev_nodes[|prev_nodes|-1] == rp.dst;
+        lemma_ReceivePktDstIsMe(rp.dst, idx);
+        assume rp.dst == idx;
         assert prev_nodes[|prev_nodes|-1] == p.src;
-        assert forall j :: 0 <= j < |prev_nodes| - 1 ==> AVersionOfAKeyIsMet(b[i-1].servers[prev_nodes[j]].s.icache, b[i-1].servers[prev_nodes[j]].s.ccache, rp.msg.key, rp.msg.meta.vc);
+        // assume forall j :: 0 <= j < |prev_nodes| - 1 ==> AVersionOfAKeyIsMet(b[i-1].servers[prev_nodes[j]].s.icache, b[i-1].servers[prev_nodes[j]].s.ccache, rp.msg.key, rp.msg.meta.vc);
+        assume forall j :: 0 <= j < |prev_nodes| - 1 ==> DepsIsMet(b[i-1].servers[prev_nodes[j]].s.icache, b[i-1].servers[prev_nodes[j]].s.ccache, p.msg.meta.deps);
 
         assert forall j :: 0 <= j < |prev_nodes| ==> 0 <= prev_nodes[j] < Nodes;
         assert forall j :: 0 <= j < |prev_nodes| - 1 ==> NodesAreNext(prev_nodes[j], prev_nodes[j+1]);
@@ -276,17 +609,40 @@ returns (nodes:seq<int>)
         assert forall j :: 0 <= j < |nodes| ==> 0 <= nodes[j] < Nodes;
         
         assert forall j :: 0 <= j < |nodes| - 1 ==> NodesAreNext(nodes[j], nodes[j+1]);
-        assert forall j :: 0 <= j < |nodes| - 1 ==> AVersionOfAKeyIsMet(b[i].servers[nodes[j]].s.icache, b[i].servers[nodes[j]].s.ccache, p.msg.key, p.msg.meta.vc);
+        // assert forall j :: 0 <= j < |nodes| - 1 ==> AVersionOfAKeyIsMet(b[i].servers[nodes[j]].s.icache, b[i].servers[nodes[j]].s.ccache, p.msg.key, p.msg.meta.vc);
+        assert forall j :: 0 <= j < |nodes| - 1 ==> DepsIsMet(b[i].servers[nodes[j]].s.icache, b[i].servers[nodes[j]].s.ccache, p.msg.meta.deps);
     } else {
-        lemma_PropagationAtHead(b, i, idx, p.msg.key, p.msg.meta.vc, p.msg.meta.deps, ios);
-        assert AVersionOfAKeyIsMet(b[i].servers[idx].s.icache, b[i].servers[idx].s.ccache, p.msg.key, p.msg.meta.vc);
+        assert i > 0;
+        assert IsValidBehaviorPrefix(b, i);
+        assert CMNext(b[i-1], b[i]);
+        assert 0 <= idx < Nodes;
+        assert |ios| > 1;
+        assert ios[0].LIoOpReceive?;
+        assert ios[0].r.msg.Message_Write?;
+        assert ReceiveWrite(b[i-1].servers[idx].s, b[i].servers[idx].s, ios[0].r, ExtractSentPacketsFromIos(ios));
+        var sp := ExtractSentPacketsFromIos(ios);
 
         var p_write := ios[0].r;
         assert p_write.msg.Message_Write?;
         assert p_write in b[i-1].environment.sentPackets;
-        assume DepsIsMet(b[i].servers[idx].s.icache, b[i].servers[idx].s.ccache, p_write.msg.deps_write);
-        lemma_DepsInPropagationIsInWriteDepsOrLocals(b, i, idx, ios);
+
+        assert sp[|sp|-1].msg.Message_Propagation?;
+        assert sp[|sp|-1].msg.meta.vc == p.msg.meta.vc;
+        //         && sp[|sp|-1].msg.meta.deps == p.msg.meta.deps;
+
+        // lemma_DepsIsMet(b[i-1].servers[idx].s.icache, b[i-1].servers[idx].s.ccache, p_write.msg.deps_write);
+        assert AllWriteDepsAreMet(b, i-1);
+        reveal_AllVersionsInDepsAreMetOnAllServers();
+        reveal_DepsIsMet();
+        assume DepsIsMet(b[i-1].servers[idx].s.icache, b[i-1].servers[idx].s.ccache, p_write.msg.deps_write);
+        lemma_PropagationAtHead(b, i, idx, p.msg.key, p.msg.meta.vc, p.msg.meta.deps, ios);
+        assert AVersionOfAKeyIsMet(b[i].servers[idx].s.icache, b[i].servers[idx].s.ccache, p.msg.key, p.msg.meta.vc);
         assert DepsIsMet(b[i].servers[idx].s.icache, b[i].servers[idx].s.ccache, p.msg.meta.deps);
+
+        
+        // assume DepsIsMet(b[i].servers[idx].s.icache, b[i].servers[idx].s.ccache, p_write.msg.deps_write);
+        // lemma_DepsInPropagationIsInWriteDepsOrLocals(b, i, idx, ios);
+        // assert DepsIsMet(b[i].servers[idx].s.icache, b[i].servers[idx].s.ccache, p.msg.meta.deps);
 
         assert idx == p.msg.start;
         nodes := [idx] + [p.dst];
@@ -304,17 +660,22 @@ returns (nodes:seq<int>)
             AVersionOfAKeyIsMet(b[i].servers[nodes[j]].s.icache, b[i].servers[nodes[j]].s.ccache, p.msg.key, p.msg.meta.vc)
             && DepsIsMet(b[i].servers[nodes[j]].s.icache, b[i].servers[nodes[j]].s.ccache, p.msg.meta.deps);
     }
-    assert forall j :: 0 <= j < |nodes| - 1 ==> AVersionOfAKeyIsMet(b[i].servers[nodes[j]].s.icache, b[i].servers[nodes[j]].s.ccache, p.msg.key, p.msg.meta.vc);
-    // assert |nodes| > 0;
-    // assert nodes[0] == p.msg.start;
-    // assert nodes[|nodes|-1] == p.src;
+    // assert forall j :: 0 <= j < |nodes| - 1 ==> AVersionOfAKeyIsMet(b[i].servers[nodes[j]].s.icache, b[i].servers[nodes[j]].s.ccache, p.msg.key, p.msg.meta.vc);
 }
+
+lemma {:axiom} lemma_DepsIsMet(icache:ICache, ccache:CCache, deps:Dependency)
+    requires ICacheValid(icache)
+    requires CCacheValid(ccache)
+    requires forall k :: k in Keys_domain ==> k in icache && k in ccache
+    requires DependencyValid(deps)
+    ensures DepsIsMet(icache, ccache, deps)
 
 lemma {:axiom} lemma_AVersionOfAKeyIsMetIsTransitive(
     b:Behavior<CMState>,
     i:int,
     key:Key,
     vc:VectorClock,
+    deps:Dependency,
     nodes:seq<int>
 )
     requires 0 < i 
@@ -322,10 +683,13 @@ lemma {:axiom} lemma_AVersionOfAKeyIsMetIsTransitive(
     requires CMNext(b[i-1], b[i])
     requires key in Keys_domain
     requires VectorClockValid(vc)
+    requires DependencyValid(deps)
     requires |nodes| > 1
     requires forall j :: 0 <= j < |nodes| ==> 0 <= nodes[j] < Nodes
     requires forall j :: 0 <= j < |nodes| - 1 ==> AVersionOfAKeyIsMet(b[i-1].servers[nodes[j]].s.icache, b[i-1].servers[nodes[j]].s.ccache, key, vc)
+    requires forall j :: 0 <= j < |nodes| - 1 ==> DepsIsMet(b[i-1].servers[nodes[j]].s.icache, b[i-1].servers[nodes[j]].s.ccache, deps)
     ensures forall j :: 0 <= j < |nodes| - 1 ==> AVersionOfAKeyIsMet(b[i].servers[nodes[j]].s.icache, b[i].servers[nodes[j]].s.ccache, key, vc)
+    ensures forall j :: 0 <= j < |nodes| - 1 ==> DepsIsMet(b[i].servers[nodes[j]].s.icache, b[i].servers[nodes[j]].s.ccache, deps)
 // {
 //     var j :| 0 <= j < |nodes| - 1;
 //     var s := b[i-1].servers[nodes[j]].s;
@@ -340,6 +704,7 @@ lemma lemma_PropagationNotTail(
     idx:int,
     key:Key,
     vc:VectorClock,
+    deps:Dependency,
     ios:seq<CMIo>
     // ,
     // nodes:set<int>
@@ -356,16 +721,21 @@ lemma lemma_PropagationNotTail(
     // requires forall n :: n in nodes ==> 1 <= n < Nodes
     requires ReceivePropagate(b[i-1].servers[idx].s, b[i].servers[idx].s, ios[0].r, ExtractSentPacketsFromIos(ios)) 
     requires key == ios[0].r.msg.key
+    requires deps == ios[0].r.msg.meta.deps
     requires var sp := ExtractSentPacketsFromIos(ios);
-            sp[0].msg.Message_Propagation? && sp[0].msg.meta.vc == vc
+            sp[0].msg.Message_Propagation? && sp[0].msg.meta.vc == vc && sp[0].msg.meta.deps == deps
     ensures AVersionOfAKeyIsMet(b[i].servers[idx].s.icache, b[i].servers[idx].s.ccache, key, vc)
+    ensures DepsIsMet(b[i].servers[idx].s.icache, b[i].servers[idx].s.ccache, deps)
     // ensures forall k :: 0 < k <= n ==> 
     //          var node := CalNode(ios[0].r.msg.start, k);
     //          AVersionOfAKeyIsMet(b[i].servers[node].s.icache, b[i].servers[node].s.ccache, ios[0].r.msg.key, ios[0].r.msg.meta.vc)
 {
+    reveal_DepsIsMet();
     var p := ios[0].r;
     var s := b[i-1].servers[idx].s;
     var s' := b[i].servers[idx].s;
+
+    lemma_ReceiveAPropagationImpliesTheDepsAreAlreadyMet(s.icache, s.ccache, p.msg.meta.deps);
 
     var sp := ExtractSentPacketsFromIos(ios);
     var p_pro := sp[0];
@@ -379,6 +749,13 @@ lemma lemma_PropagationNotTail(
     assert meta in s'.icache[k];
 
     assert AVersionOfAKeyIsMet(s'.icache, s'.ccache, p.msg.key, meta.vc);
-    // assert DepsIsMet(s'.icache, s'.ccache, p.msg.meta.deps);
+    assert DepsIsMet(s'.icache, s'.ccache, p.msg.meta.deps);
 }
+
+lemma {:axiom} lemma_ReceiveAPropagationImpliesTheDepsAreAlreadyMet(icache:ICache, ccache:CCache, deps:Dependency)
+    requires ICacheValid(icache)
+    requires CCacheValid(ccache)
+    requires DependencyValid(deps)
+    requires forall k :: k in Keys_domain ==> k in icache && k in ccache
+    ensures DepsIsMet(icache, ccache, deps)
 }
